\subsection{Proof of Lifted Retract (Lemma~\ref{lemma:lifted_retract})}
\label{subsec:proof_of_lifted_retract}
This is a proof by induction on the form of $[[A]]$.

\begin{itemize}
\item[] Case. Suppose $[[A]]$ is atomic.  Then:
  \[
    [[lbox A]];[[lunbox A]] = [[box A]];[[unbox A]] = \id_{[[A]]}
    \]
    
  \item[] Case. Suppose $[[A]]$ is $[[?]]$.  Then:
    \[
    \begin{array}{lll}
      [[lbox A]];[[lunbox A]] & = & [[lbox ?]];[[lunbox ?]]\\
      & = & \id_{[[?]]};\id_{[[?]]}\\
      & = & \id_{[[?]]}\\
      & = & \id_{[[A]]}
    \end{array}
    \]

  \item[] Case. Suppose $[[A]] = [[A1 -> A2]]$.  Then:
    \[\small
    \begin{array}{lll}
      [[lbox A]];[[lunbox A]]
      & = & [[lbox (A1 -> A2)]];[[lunbox (A1 -> A2)]]\\
      & = & ([[lunbox A1]] \to [[lbox A2]]);([[lbox A1]] \to [[lbox A2]])\\
      & = & ([[lbox A1]];[[lunbox A1]]) \to ([[lbox A2]];[[lunbox A2]])\\
    \end{array}
    \]
    By two applications of the induction hypothesis we know the
    following:
    \[
    \begin{array}{lll}
      [[lbox A1]];[[lunbox A1]] = \id_{[[A1]]} & \text{ and } & [[lbox A2]];[[lunbox A2]] = \id_{[[A2]]}
    \end{array}
    \]
    Thus, we know the following:
    \[
    \begin{array}{lll}
      ([[lbox A1]];[[lunbox A1]]) \to ([[lbox A2]];[[lunbox A2]])
      & = & \id_{[[A1]]} \to \id_{[[A2]]}\\
      & = & \id_{[[A1 -> A2]]}\\
      & = & \id_{[[A]]}
    \end{array}
    \]

  \item[] Case. Suppose $[[A]] = [[A1 x A2]]$.  Then:
    \[\small
    \begin{array}{lll}
      [[lbox A]];[[lunbox A]]
      & = & [[lbox (A1 x A2)]];[[lunbox (A1 x A2)]]\\
      & = & ([[lbox A1]] \times [[lbox A2]]);([[lunbox A1]] \times [[lbox A2]])\\
      & = & ([[lbox A1]];[[lunbox A1]]) \times ([[lbox A2]];[[lunbox A2]])\\
    \end{array}
    \]
    By two applications of the induction hypothesis we know the
    following:
    \[
    \begin{array}{lll}
      [[lbox A1]];[[lunbox A1]] = \id_{[[A1]]} & \text{ and } & [[lbox A2]];[[lunbox A2]] = \id_{[[A2]]}
    \end{array}
    \]
    Thus, we know the following:
    \[
    \begin{array}{lll}
      ([[lbox A1]];[[lunbox A1]]) \times ([[lbox A2]];[[lunbox A2]])
      & = & \id_{[[A1]]} \times \id_{[[A2]]}\\
      & = & \id_{[[A1 x A2]]}\\
      & = & \id_{[[A]]}
    \end{array}
    \]
\end{itemize}
% subsection proof_of_lifted_retract (end)

\subsection{Proof of Lemma~\ref{lemma:S_is_faithful}}
\label{subsec:proof_of_S_is_faithful}
We must show that the function
  \[ \S_{A,B} : \Hom{C}{A}{B} \mto \Hom{S}{\S A}{\S B} \]
  is injective.

  So suppose $f \in \Hom{C}{A}{B}$ and $g \in \Hom{C}{A}{B}$ such that
  $\S f = \S g : \S A \mto \S B$.  Then we can easily see that:
  \[
  \begin{array}{lll}
    \S f & = & [[lunbox A]];f;[[lbox B]] \\
         & = & [[lunbox A]];g;[[lbox B]]\\
         & = & \S g\\
  \end{array}
  \]
  But, we have the following equalities:
  \[\scriptsize
  \begin{array}{rll}
    [[lunbox A]];f;[[lbox B]] & = & [[lunbox A]];g;[[lbox B]]\\
    [[lbox A]];[[lunbox A]];f;[[lbox B]];[[lunbox B]] & = & [[lbox A]];[[lunbox A]];g;[[lbox B]];[[lunbox B]]\\
    \id_A;f;[[lbox B]];[[lunbox B]] & = & \id_A;g;[[lbox B]];[[lunbox B]]\\
    \id_A;f;\id_B & = & \id_A;g;\id_B\\
    f & = & g\\
  \end{array}
  \]
  The previous equalities hold due to
  Lemma~\ref{lemma:lifted_retract}.
% subsection proof_of_S_is_faithful (end)

%%% Local Variables: ***
%%% mode:latex ***
%%% TeX-master: "main.tex"  ***
%%% End: ***
